pcuic/theories/PCUICAst.v
@@ -15,7 +15,7 @@ Open Scope pcuic.
    In particular, it has binary applications and all terms are well-formed.
    Casts are absent as well. *)
 
-Inductive term : Set :=
+Inductive term :=
 | tRel (n : nat)
 | tVar (i : ident) (* For free variables (e.g. in a goal) *)
 | tEvar (n : nat) (l : list term)
@@ -93,11 +93,11 @@ Inductive constant_entry :=
   [x1:X1;...;xn:Xn].
 *)
 
-Inductive local_entry : Set :=
+Inductive local_entry :=
 | LocalDef : term -> local_entry (* local let binding *)
 | LocalAssum : term -> local_entry.
 
-Record one_inductive_entry : Set := {
+Record one_inductive_entry := {
   mind_entry_typename : ident;
   mind_entry_arity : term;
   mind_entry_template : bool; (* template polymorphism *)
